@prefix coso: <http://w3id.org/coso/v1/contaminoso#> .
@prefix dsstox: <http://w3id.org/DSSTox/v1/>.
@prefix geo: <http://www.opengis.net/ont/geosparql#> .
@prefix owl: <http://www.w3.org/2002/07/owl#> .
@prefix rdf: <http://www.w3.org/1999/02/22-rdf-syntax-ns#> .
@prefix xml: <http://www.w3.org/XML/1998/namespace> .
@prefix xsd: <http://www.w3.org/2001/XMLSchema#> .
@prefix rdfs: <http://www.w3.org/2000/01/rdf-schema#> .
@prefix qudt: <http://qudt.org/schema/qudt/> .
@prefix sosa: <http://www.w3.org/ns/sosa/> .
@prefix dcterms: <http://purl.org/dc/terms/> .
@prefix vann: <http://purl.org/vocab/vann/> .
@base <http://w3id.org/coso/comptox_ext#> .

<http://w3id.org/coso/dsstox_ext#> rdf:type owl:Ontology ;
                                              owl:versionIRI <http://w3id.org/coso/v1/comptox_ext#> ;
                                              dcterms:created "2025-03-30"@en-us ;
                                              dcterms:creator <http://orcid.org/0000-0002-5331-5052> ,
                                                              <http://orcid.org/0000-0003-3547-8058> ,
                                                              <https://orcid.org/0000-0003-3271-6700> ;
                                              dcterms:description "the Contaminant Observation and Samples Ontology (ContaminOSO) extension to support DSSTox substance."@en-us ;
                                              dcterms:abstract "";
                                              dcterms:issued "2025-03-30"^^xsd:date ;
                                              dcterms:modified "2025-03-30"^^xsd:date ;
                                              dcterms:publisher <http://spatialai.org> ;
                                              dcterms:source "https://raw.githubusercontent.com/SAWGraph/kg-construction/master/ontologies/v1/contaminoso_dsstox_ext.ttl"^^<xsd:anyURI> ;
                                              dcterms:title "Contaminant Observation and Samples Ontology"@en-us ;
                                              rdfs:label "ContaminOSO"@en-us ;
                                              vann:preferredNamespaceUri <http://w3id.org/coso/v1/dsstox_ext#>;
                                              vann:preferredNamespacePrefix "coso_dsstox:";
                                              owl:versionInfo "1"@en-us .

coso:ofDSSToxSubstance a owl:ObjectProperty;
        rdfs:label "of DSSTox Substance";
        dcterms:description "A relation between an entity and a chemical substance as identified by DSSTox";
        rdfs:subPropertyOf coso:ofSubstance;
        rdfs:range dsstox:ChemicalEntity;
        owl:propertyChainAxiom (coso:ofDatasetSubstance dsstox:sameAsDSSToxSubstance).  

coso:ofDatasetSubstance a owl:ObjectProperty;
        rdfs:label "of Dataset Substance";
        dcterms:description "A relation between an entity and a chemical substance as identified in a dataset specific controlled vocabulary";
        rdfs:subPropertyOf coso:ofSubstance.
        #range is disjoint with dsstox:CheimcalEntity.   

dsstox:sameAsDSSToxSubstance a owl:ObjectProperty;
    rdfs:label "same as DSSTox substance";
    dcterms:description "A relation between an dataset specific substance and the same substance as identified in dsstox.";
    rdfs:range dsstox:ChemicalEntity. 

dsstox:ChemicalEntity rdf:type owl:Class;
    rdfs:subClassOf coso:Substance.