@prefix coso: <http://w3id.org/coso/v1/contaminoso#> .
@prefix geo: <http://www.opengis.net/ont/geosparql#> .
@prefix owl: <http://www.w3.org/2002/07/owl#> .
@prefix rdf: <http://www.w3.org/1999/02/22-rdf-syntax-ns#> .
@prefix xml: <http://www.w3.org/XML/1998/namespace> .
@prefix xsd: <http://www.w3.org/2001/XMLSchema#> .
@prefix rdfs: <http://www.w3.org/2000/01/rdf-schema#> .
@prefix qudt: <http://qudt.org/schema/qudt/> .
@prefix sosa: <http://www.w3.org/ns/sosa/> .
@prefix dcterms: <http://purl.org/dc/terms/> .
@prefix vann: <http://purl.org/vocab/vann/> .
@base <http://w3id.org/coso/contaminoso#> .

<http://w3id.org/coso/contaminoso#> rdf:type owl:Ontology ;
                                              owl:versionIRI coso: ;
                                              dcterms:created "2025-03-30"@en-us ;
                                              dcterms:creator <http://orcid.org/0000-0002-5331-5052> ,
                                                              <http://orcid.org/0000-0003-3547-8058> ,
                                                              <https://orcid.org/0000-0003-3271-6700> ;
                                              dcterms:description "the Contaminant Observation and Samples Ontology (ContaminOSO) developed as part of the AIKnowsPFAS and SAWGraph projects."@en-us ;
                                              dcterms:abstract "";
                                              dcterms:issued "2025-03-30"^^xsd:date ;
                                              dcterms:modified "2025-03-30"^^xsd:date ;
                                              dcterms:publisher <http://spatialai.org> ;
                                              dcterms:source "https://raw.githubusercontent.com/SAWGraph/kg-construction/master/ontologies/v1/contaminoso.ttl"^^<xsd:anyURI> ;
                                              dcterms:title "Contaminant Observation and Samples Ontology"@en-us ;
                                              rdfs:label "ContaminOSO"@en-us ;
                                              vann:preferredNamespaceUri <http://w3id.org/coso/contaminoso#>;
                                              vann:preferredNamespacePrefix "coso:";
                                              owl:versionInfo "1"@en-us .

#################################################################
#    Annotation properties
#################################################################

dcterms:created rdf:type owl:AnnotationProperty .

dcterms:creator rdf:type owl:AnnotationProperty .

dcterms:description rdf:type owl:AnnotationProperty .

dcterms:issued rdf:type owl:AnnotationProperty .

dcterms:modified rdf:type owl:AnnotationProperty .

dcterms:publisher rdf:type owl:AnnotationProperty .

dcterms:source rdf:type owl:AnnotationProperty .

dcterms:title rdf:type owl:AnnotationProperty .


#################################################################
#    Datatypes
#################################################################

###  http://www.w3.org/2001/XMLSchema#date
xsd:date rdf:type rdfs:Datatype .


###  xsd:anyURI
<xsd:anyURI> rdf:type rdfs:Datatype .


#################################################################
#    Classes
#################################################################

coso:ContaminantObservation rdf:type owl:Class ;
    rdfs:label "Contaminant Observation" ;
    dcterms:description "An observation of a contaminant." ;
    rdfs:subClassOf sosa:Observation .

coso:ContaminantReleaseObservation rdf:type owl:Class ;
    rdfs:label "Contaminant Release Observation" ;
    dcterms:description "An observation of a contaminant that was released into the environment.";
    rdfs:subClassOf coso:ContaminantObservation .

coso:ContaminantSampleObservation rdf:type owl:Class ;
    rdfs:label "Contaminant Sample Observation" ;
    dcterms:description "An observation of a contaminant that was sampled from the environment. ";
    rdfs:subClassOf coso:ContaminantObservation .

coso:Feature rdf:type owl:Class ;
    rdfs:label "Feature" ;
    dcterms:description "The discrete spatial phenomenon that is the target of the observation. " ;
    rdfs:subClassOf geo:Feature ,
                    sosa:FeatureOfInterest .

coso:FeatureType rdf:type owl:Class ;
    rdfs:label "Feature Type" ;
    dcterms:description "A category applied to differentiate discrete spatial phenomenon. ". 

coso:SampledFeature rdf:type owl:Class ;
    rdfs:label "Sampled Feature" ;
    dcterms:description "The discrete spatial phenomenon that is the target of a sample observation. ";
    rdfs:subClassOf coso:Feature .

coso:ReleaseFeature rdf:type owl:Class ;
    rdfs:label "Release Feature" ;
    dcterms:description "The discrete spatial phenomenon that may be the target of a release observation. ";
    rdfs:subClassOf coso:Feature .

coso:MonitoredFeature rdf:type owl:Class ;
    rdfs:label "Monitored Feature" ;
    dcterms:description "The discrete spatial phenomenon that is the target of a release observation due to environmental monitoring. ";
    rdfs:subClassOf coso:ReleaseFeature .

coso:Point rdf:type owl:Class ;
    rdfs:label "Point" ;
    dcterms:description "The point location at which an observation occurred.";
    rdfs:subClassOf geo:Feature ,
                    sosa:FeatureOfInterest .

coso:SamplePoint rdf:type owl:Class ;
    rdfs:label "Sample Point" ;
    dcterms:description "The point location at which a sample observation occurred.";
    rdfs:subClassOf coso:Point .

coso:ReleasePoint rdf:type owl:Class ;
    rdfs:label "Release Point" ;
    dcterms:description "The point location at which a release observation occurred.";
    rdfs:subClassOf coso:Point .

coso:MaterialSample rdf:type owl:Class ;
    rdfs:label "Material Sample" ;
    dcterms:description "A physical, tangible sample." ;
    rdfs:subClassOf sosa:Sample .

coso:SampleMaterialType rdf:type owl:Class ;
    rdfs:label "Sample Material Type" ;
    dcterms:description "The type of material that was sampled".

coso:AnalysisMethod rdf:type owl:Class ;
    rdfs:label "Analysis Method" ;
    dcterms:description "The analysis method used to identify the contaminant."; 
    rdfs:subClassOf sosa:Procedure .

coso:ContaminationProperty rdf:type owl:Class ;
    rdfs:label "Contamination Property" ;
    dcterms:description "An observable quality of a feature related to its contamination. "; 
    rdfs:subClassOf sosa:Property .

coso:ContaminantAbsoluteQuantityKind rdf:type owl:Class ;
    rdfs:label "Contaminant Absolute Quantity Kind" ;
    dcterms:description "A type of contaminant quantity that is an absolute amount, such as a mass or volume.";
    rdfs:subClassOf coso:ContaminationProperty .

coso:ContaminantRelativeQuantityKind rdf:type owl:Class ;
    rdfs:label "Contaminant Relative Quantity Kind" ;
     dcterms:description "A type of contaminant quantity that is a relative amount, such as a concentration.";
    rdfs:subClassOf coso:ContaminationProperty .

coso:ContaminantMassQuantityKind rdf:type owl:Class ;
    rdfs:label "Contaminant Quantity Kind" ;
    dcterms:description "The type of quantity that is measured for the contaminant.";
    rdfs:subClassOf coso:ContaminantAbsoluteQuantityKind .

coso:ContaminantVolumeQuantityKind rdf:type owl:Class ;
    rdfs:label "Contaminant Volume Quantity Kind" ;
    dcterms:description "A type of contaminant quantity that is a volume measurement.";
    rdfs:subClassOf coso:ContaminantAbsoluteQuantityKind .

coso:ContaminantConcentrationQuantityKind rdf:type owl:Class ;
    rdfs:label "Contaminant Concentration Quantity Kind" ;
    dcterms:description "A type of contaminant quantity that is a concentration measurement.";
    rdfs:subClassOf coso:ContaminantRelativeQuantityKind.

coso:ContaminantMeasurement rdf:type owl:Class ;
    rdfs:label "Contaminant Measurement" ;
    dcterms:description "The result of an observation about a contaminant or contaminants." ;
    rdfs:subClassOf sosa:Result .

coso:ContaminantAbsoluteMeasurement rdf:type owl:Class ;
    rdfs:label "Contaminant Absolute Measurement" ;
    dcterms:description "The result of an observation about a contaminant that is an absolute measurement." ;
    rdfs:subClassOf coso:ContaminantMeasurement .

coso:ContaminantRelativeMeasurement rdf:type owl:Class ;
    rdfs:label "Contaminant Relative Measurement" ;
    dcterms:description "The result of an observation about a contaminant that is a relative measurement." ;
    rdfs:subClassOf coso:ContaminantMeasurement .

coso:AggregateContaminantMeasurement rdf:type owl:Class ;
    rdfs:label "Aggregate Contaminant Measurement";
    dcterms:description "The result of an observation about contaminant(s) that is an aggregate measurement. This can be a spatial, temporal or contaminant aggregate." ;
    rdfs:subClassOf coso:ContaminantMeasurement .

coso:SingleContaminantMeasurement rdf:type owl:Class ;
    rdfs:label "Single Contaminant Measurement" ;
    dcterms:description "The result of an observation about a contaminant that is a single measurement, i.e. a single contaminant at one location from one sample." ;
    rdfs:subClassOf coso:ContaminantMeasurement .

coso:QuantityValue rdf:type owl:Class;
    dcterms:description "A Quantity Value expresses the magnitude and kind of a quantity as a product of a numerical value or enumerated value and a unit of measure." ;
    rdfs:label "Quantity Value" .

coso:DetectQuantityValue rdf:type owl:Class ;
    rdfs:label "Detect Quantity Value" ;
    dcterms:description "A Quantity Value that represents a detection of the contaminant.";
    rdfs:subClassOf coso:QuantityValue .

coso:NonDetectQuantityValue rdf:type owl:Class ;
    rdfs:label "Non-Detect Quantity Value" ;
    dcterms:description "A Quantity Value that represents a non-detection of the contaminant. No numeric value is specified.";
    rdfs:subClassOf coso:QuantityValue .

coso:ResultQualifier rdf:type owl:Class ;
    rdfs:label "Result Qualifier"; 
    dcterms:description "Something that qualifies the result, such as quality control assessment, limitation on the precision or minimum detectable amount. ".

coso:DetectionLimit rdf:type owl:Class ;
    rdfs:label "Detection Limit" ;
    dcterms:description "The lowest concentration of a substance that can be reliably detected as present with a reasonable degree of confidence.";
    rdfs:subClassOf coso:ResultQualifier .

coso:QuantitationLimit rdf:type owl:Class ;
    rdfs:label "Quantitation Limit" ;
    dcterms:description "The lowest concentration of a substance that can be reliably measured with acceptable precision and accuracy.";
    rdfs:subClassOf coso:ResultQualifier .

coso:ObservationAnnotation rdf:type owl:Class ;
    rdfs:label "Observation Annotation";
    dcterms:description "Metadata that qualifies an observation".

coso:SampleAnnotation rdf:type owl:Class ;
    rdfs:label "Sample Annotation"; 
    dcterms:description "Metadata that qualifies a sample".

coso:Substance rdf:type owl:Class ;
    rdfs:label "Substance";
    dcterms:description "Any organic or inorganic substance of a particular molecular identity, including any combination of these substances occurring in whole or in part as a result of a chemical reaction or occurring in nature, and any element or uncombined radical.".

coso:SubstanceCollection rdf:type owl:Class ;
    rdfs:label "Substance Collection" ;
    dcterms:description "A collection of more than one substances.";
    rdfs:subClassOf [ rdf:type owl:Restriction ;
                        owl:onProperty rdfs:member ;
                        owl:allValuesFrom coso:Substance
                    ] .

## Reused Classes
sosa:Observation rdf:type owl:Class. 

geo:Feature rdf:type owl:Class.

sosa:FeatureOfInterest rdf:type owl:Class. 

sosa:Sample rdf:type owl:Class. 

sosa:Procedure rdf:type owl:Class. 

sosa:Property rdf:type owl:Class. 

sosa:Result rdf:type owl:Class. 

#################################################################
#    Object Properties
#################################################################

coso:hasAnyFeatureOfInterest rdf:type owl:ObjectProperty ;
    rdfs:label "has any feature of interest";
    dcterms:description "A relation between an observation of a contaminant and a feature it is the subject of. There are no specific scale or cardinality constraints that limit the feature."; 
    rdfs:domain coso:ContaminantObservation ;
    rdfs:range sosa:FeatureOfInterest .

coso:analyzedSample rdf:type owl:ObjectProperty ;
    rdfs:label "analyzed sample";
    dcterms:description "A relation between an observation of a contaminant and the sample that was analyzed."; 
    rdfs:subPropertyOf coso:hasAnyFeatureOfInterest ;
    rdfs:domain coso:ContaminantSampleObservation ;
    rdfs:range coso:MaterialSample .

coso:hasFeatureOfInterest rdf:type owl:ObjectProperty ;
    rdfs:label "has feature of interest";
    dcterms:description "A relation between an observation of a contaminant and a feature it is the subject of.";
    rdfs:subPropertyOf coso:hasAnyFeatureOfInterest ;
    rdfs:range coso:Feature .

coso:sampledFeature rdf:type owl:ObjectProperty ;
    rdfs:label "sampled feature";
    dcterms:description "A relation between an observation of a contaminant from a sample and the feature that was sampled.";
    rdfs:subPropertyOf coso:hasFeatureOfInterest ;
    rdfs:domain coso:ContaminantSampleObservation ;
    rdfs:range coso:SampledFeature .

coso:releaseFeature rdf:type owl:ObjectProperty ;
    rdfs:label "release feature";
    rdfs:subPropertyOf coso:hasFeatureOfInterest ;
    dcterms:description "A relation between an observation of a contaminant that was released and the feature where it was released.";
    rdfs:domain coso:ContaminantReleaseObservation ;
    rdfs:range coso:ReleaseFeature .

coso:observedAtPoint rdf:type owl:ObjectProperty ;
    rdfs:label "observed at point";
    rdfs:subPropertyOf coso:hasAnyFeatureOfInterest ;
    dcterms:description "A relation between an observation of a contaminant and the point that the observation applies to.";
    rdfs:domain coso:ContaminantObservation ;
    rdfs:range coso:Point .

coso:observedAtReleasePoint rdf:type owl:ObjectProperty ;
    rdfs:label "observed at release point";
    dcterms:description "A relation between an observation of a contaminant that was released and the point where the observation was made and where the release occurred.";
    rdfs:subPropertyOf coso:observedAtPoint ;
    rdfs:domain coso:ContaminantReleaseObservation ;
    rdfs:range coso:ReleasePoint .

coso:observedAtSamplePoint rdf:type owl:ObjectProperty ;
    rdfs:label "observed at sample point";
    dcterms:description "A relation between an observation of a contaminant from a material sample and the point where the sample was taken.";
    rdfs:subPropertyOf coso:observedAtPoint ;
    rdfs:domain coso:ContaminantSampleObservation ;
    rdfs:range coso:SamplePoint .

coso:fromSamplePoint rdf:type owl:ObjectProperty ;
    rdfs:label "from sample point";
    dcterms:description "A relation between a physical material sample and the location where the sample was taken.";
    rdfs:domain coso:MaterialSample ;
    rdfs:range coso:SamplePoint .

coso:isSampleOf rdf:type owl:ObjectProperty ;
    rdfs:label "is sample of";
    dcterms:description "A relation between a physcial material sample and the geographic feature the sample was taken from.";
    rdfs:subPropertyOf sosa:isSampleOf ;
    rdfs:domain coso:MaterialSample ;
    rdfs:range coso:SampledFeature .

coso:hasResult rdf:type owl:ObjectProperty ;
    rdfs:label "has result";
    dcterms:description "A relation between an observation of a contaminant and the measurement that is the result of the observation.";
    rdfs:subPropertyOf sosa:hasResult;
    rdfs:domain coso:ContaminantObservation;
    rdfs:range coso:ContaminantMeasurement.

coso:hasResultQualifier rdf:type owl:ObjectProperty ;
    rdfs:label "has result qualifier";
    dcterms:description "A relation between measured result and metadata that qualifies the result.";
    rdfs:domain coso:ContaminantMeasurement;
    rdfs:range coso:ResultQualifier .

coso:pointFromFeature rdf:type owl:ObjectProperty ;
    rdfs:label "point from feature";
    dcterms:description "A relation between a point location and the larger geospatial feature it is a part of.";
    rdfs:domain coso:Point ;
    rdfs:range coso:Feature .

coso:observationAnnotation rdf:type owl:ObjectProperty ;
    rdfs:label "observation annotation";
    dcterms:description "A relation between an observation of a contaminant and additional metadata about the observation.";
    rdfs:domain coso:ContaminantObservation;
    rdfs:range coso:ObservationAnnotation.

coso:observedProperty rdf:type owl:ObjectProperty ;
    rdfs:label "observed property";
    dcterms:description "A relation between an observation and the type of contamination property being observed. ";
    rdfs:subPropertyOf sosa:observedProperty ;
    rdfs:domain coso:ContaminantObservation ;
    rdfs:range coso:ContaminationProperty .

coso:ofSubstance rdf:type owl:ObjectProperty ;
    rdfs:label "of substance";
    dcterms:description "A relation between an observation of a contaminant and the substance or substances being observed.";
    rdfs:domain coso:ContaminantObservation ;
    rdfs:range [ rdf:type owl:Class ;
                 owl:unionOf ( coso:Substance
                               coso:SubstanceCollection
                              )
                ] .

coso:ofFeatureType rdf:type owl:ObjectProperty ;
    rdfs:label "of feature type";
    dcterms:description "A relation between a feature and a controlled vocabulary term that describes the type of feature";
    rdfs:range coso:FeatureType. 

coso:resultAnnotation rdf:type owl:ObjectProperty ;
    rdfs:label "result annotation"; 
    dcterms:description "A relation between a result and additional metadata about the result.".

coso:sampleAnnotation rdf:type owl:ObjectProperty ;
    rdfs:label "sample annotation";
    dcterms:description "A relation between a material sample and additional metadata about the sample.";
    rdfs:domain coso:MaterialSample;
    rdfs:range coso:SampleAnnotation. 


coso:sampleOfMaterialType rdf:type owl:ObjectProperty ;
    rdfs:label "sample of material type";
    dcterms:description "A relation between a material sample and the type of material.";
    rdfs:domain coso:MaterialSample ;
    rdfs:range coso:SampleMaterialType .

coso:usedAnalysisMethod rdf:type owl:ObjectProperty ;
    rdfs:label "used analysis method";
    dcterms:description "A relation between an observation of a contaminant and the analysis method that was used to perform the observation.";
    rdfs:subPropertyOf sosa:usedProcedure ;
    rdfs:domain coso:ContaminantObservation ;
    rdfs:range coso:AnalysisMethod .

###  Reused Object Properties

sosa:hasFeatureOfInterest rdf:type owl:ObjectProperty. 

sosa:isSampleOf rdf:type owl:ObjectProperty. 

sosa:hasResult rdf:type owl:ObjectProperty. 

sosa:observedProperty rdf:type owl:ObjectProperty. 

sosa:usedProcedure rdf:type owl:ObjectProperty. 
#################################################################
#    Data properties
#################################################################

coso:substanceID rdf:type owl:DatatypeProperty;
    rdfs:label "substance identifier" ;
    dcterms:description "The unique identifier for the substance.";
    rdfs:subPropertyOf dcterms:identifier. 

coso:casNumber rdf:type owl:DatatypeProperty ;
    rdfs:subPropertyOf coso:substanceID ;
    dcterms:description "The cas number of the substance.";
    rdfs:label "cas number" .

coso:measurementUnit rdf:type owl:DatatypeProperty ;
    rdfs:label "measurement unit" ;
    dcterms:description "The unit of measurement the describes the result.";
    rdfs:domain coso:ContaminantMeasurement.

coso:measurementValue rdf:type owl:DatatypeProperty ;
    rdfs:label "measurement value" ;
    dcterms:description "The numeric value or enumerated value that quantifies or qualifies the result.";
    rdfs:domain coso:ContaminantMeasurement.

coso:observedTime rdf:type owl:DatatypeProperty ;
    rdfs:label "observed time" ;
    dcterms:description "The time at which the contaminant was observed in the environment.";
    rdfs:domain coso:ContaminantObservation. 

#################################################################
#    Individuals
#################################################################

coso:MaximumContaminantConcentrationQuantityKind rdf:type owl:NamedIndividual ,
                                                      coso:ContaminantConcentrationQuantityKind ;
                                        rdfs:label "Maximum Contaminant Concentration Quantity" .


coso:SingleContaminantConcentrationQuantityKind rdf:type owl:NamedIndividual ,
                                                     coso:ContaminantConcentrationQuantityKind ;
                                        rdfs:label "Single Contamiant Concentration Quantity" .

coso:SingleContaminantVolumeQuantityKind rdf:type owl:NamedIndividual ,
                                              coso:ContaminantVolumeQuantityKind ;
                                        rdfs:label "Single Contaminant Volume Quantity" .

coso:SummedContaminantVolumeQuantityKind rdf:type owl:NamedIndividual ,
                                              coso:ContaminantVolumeQuantityKind ;
                                        rdfs:label "Summed Contaminant Volume Quantity" .

coso:non-detect rdf:type qudt:EnumeratedValue ;
                        rdfs:label "Non-Detect";
                        dcterms:description "Non-Detect Value" ;
                        qudt:abbreviation "ND" .
